\begin{problem}
    If $x$ and $y$ are integers and $x^2+y^2$ is even, prove that $x+y$ is even.\\

    \noindent Note: You may use without proof the fact that the product of two integers is even unless both integers are odd. You may use without proof the closure properties of the integers.

    \begin{solution}
        Proof by contraposative: I will prove the contraposative of the claim by showing that both $x+y$ and $x^2+y^2$ are odd \\
        Definition: Even(x) is true if $x \in 2k; k \in \mathbb{Z}$ \\
        Definition : Odd(x) is true if $x = 2k+1; k \in \mathbb{Z}$ \\
        $Lemma_{1}$: Odd + Even = Odd $\because k_1, k_2, k_3 \in \mathbb{Z}; 2k_1 + (2k_2 + 1) = 2k_3 + 1 $ \\
        $Lemma_{2}$: Odd - Even = Odd $\because$ let $k, k_{1}, k_{2}, k_{3} \in \mathbb{Z}$; Even := $2k$; Odd:= $2k + 1$; $(2k_{1} + 1) - 2k_{1} = 2(k_{1} - k_{2}) + 1 = 2k_{3} + 1$  (Odd) \\

        Claim: $\forall (x,y \in \mathbb{Z}). Even(x^2 + y^2) \to Even(x + y)$ \\
        Contraposative: $\forall(x,y \in \mathbb{Z}). Odd(x+y) \to Odd(x^2 + y^2)$ \\

        let $k_1, k_2, x, y$ be integers \\
        $x+y = 2k_1 + 1$ \\
        $(x+y)^2 = (2k_1 + 1)^2$ \\
        $x^2 + 2xy + y^2 = 4k_1^2 + 4k_1 + 1$ \\
        $x^2 + 2xy + y^2 = 2(2k_1^2 + 2k_1) + 1$ \\
        integers are closed addition and multiplication$\therefore 2k_{1}k_{1} + 2k_1 \in \mathbb{Z}$\\
        let $k_2 := 2k_1^2 + 2k_1$ \\
        $x^2 + 2xy + y^2 = 2k_2 + 1 \therefore$ $x^2 + 2xy + y^2$ is odd \\

        $2xy$ must be even $\because$ it is the product of an even integer "2" and another (arbitrary) integer $xy$.

        Since $x^2 + 2xy + y^2$ is odd and $2xy$ is even, and the difference between an odd and even number must be odd ($Lemma_{2}$), therefore $(x^2 + 2xy + y^2) - (2xy)$ or $(x^2 + y^2)$ must be odd.



    \end{solution}
\end{problem}
\newpage

\begin{problem}
    Extend the proof of the Division Algorithm to the case of negative integers. (Note that the proof of uniqueness for non-negative numbers given in class did not depend on $a \geq 0$, so you only have to establish existence.) \\
    \emph{Hint}: Suppose $-a$ is a negative number (so $a$ is positive). From the Division Algorithm for positive integers, we already know that there are unique $q'$ and $r$ such that $a=q'd+r'$ and $0\leq r'<d$. We need to find $q$ and $r$ such that $-a=qd+r$. Consider two cases, when $r'=0$ and when $r'>0$. These examples may help:
    \begin{align}
        25=2\cdot9+7 &  & -25=(-3)\cdot 9+2 \\
        49=5\cdot 9+4 &  & -49=(-6)\cdot 9+5
    \end{align}
    \begin{solution}
        \emph{Proof.} We can will extend the proof of the Division Algorithm to the case of negative integers by showing that for any integer a and any positive integer d, there exists unique integers q and r: $a = qd + r$ and $0 \leq r < d$. \\
        Given the existing definition for the division algorithm for a positive integer $a$ such that
        $a = q'd + r'$. We can rewrite the algorithm for a negative integer $-a$ as: $-a = -(q'd + r')$ or $-a = -q'd - r'$ \\

        Case 1: $r' = 0$ \\
        $a = q'd +r$\\
        $-a = -q'd - r$ \\
        if $r' = 0$ then $-a = -q'd$ and  $r$ satisfies $0 \leq r < d \because r = 0$ \\
        and then if we let $q = -q'$ (this being a valid definition because both variables are positive/negative integers), then $-a = qd + r$. \\
        By algebraically manipulating our original proof into something which represented negative inputs, we were able to demonstrate that q and r exists which satisfy the conditions. \\

        Case 2: $r' > 0$ \\
        $-a = -q'd - r'$ \\
        $-a = -q'd - d + d - r'$ \\
        $-a = (-q(-q' + 1)d + (d - r')$ \\
        let q := -(q' + 1) and let r := (d - r') : We are able to define q and r as such because integers are closed under addition (and subtraction) and all variables involved are integers. \\
        Our definition of r satisfies $0 \leq r < d$ because $0 \leq (d - r') < d$ and $0 < r' < d$ causes the difference between d and r' to be greater than or equal to zero and less than r.

        Once we populate our original division algorithm with our new definitions we get $-a = qd + r$ showing that there exist integers q and d that satisfy the algorithm (and as a result of our definitions q', r' and their conditions). \\

        In conclusion, the proof of Division algorithm can be extended to all negative numbers by showing that the algorithm holds true for cases when r' (the remainder is equal to or when the remainder is greater than 0)
    \end{solution}
\end{problem}
\newpage

\begin{problem}
    The integers $a$ and $b$ are \emph{relatively prime} if $\textsc{GCD}(a,b) = 1$. Consider the following claim:

    \bigskip
    Prove: If, for some $x \in \mathbb{Z}$, $ax \equiv 1 \pmod{b}$, then $a$ and $b$ are relatively prime.

    \bigskip
    Note: You may find it useful to refer to the logical formulation of a very similar claim you saw in an earlier problem.

    \begin{solution}
        Proof. I will prove that for some $x \in \mathbb{Z}$, $ax \equiv 1 \pmod{b}$, then $a$ and $b$ are relatively prime. \\

        $(x \in \mathbb{Z}; ax \equiv_{b} 1) \to (a \perp b)$ \\

        Assume a and b are not co-prime. GCD(a,b) = d where d is an integer greater than 1.
        $ax \equiv 1 \mod b$ means that there exists an integer k: $ax = 1 + kb$ \\

        Since ($d \vert a$) and ($d \vert b$) we can define $a := d * a'$ and $b := d*b$' for integers a' and b'. \\
        $da'x = 1 + kdb'$ \\
        $da'x - kdb' = 1$ \\
        $d(a'x - kb') = 1$ \\
        The left hand side ($d(a'x - kb')$) is divisible by d, which means it is multiple of d. \\
        However, the right-hand side is 1, which is not divisible by d ($\because d > 1$), creating a contradiction because we cannot get 1 as a product of two integers where at least one is greater than 1.

    \end{solution}
\end{problem}
\newpage
